Sorting/MergeSort.v
@@ -200,3 +200,40 @@ Proof.
   intros. apply split'_spec1 with l2; dec.
     cbn in *. omega.
 Defined.
+
+(** Time for ultimatier mergesort. *)
+
+Class Small (A : LinDec) : Type :=
+{
+    small :> nat -> list A -> list A + A * list A;
+    small_inl :
+      forall (n : nat) (l l' : list A),
+        small n l = inl l' -> l = l';
+    small_inr :
+      forall (n : nat) (h : A) (t l : list A),
+         small n l = inr (h, t) -> Permutation l (h :: t)
+}.
+
+Coercion small : Small >-> Funclass.
+
+(* TODO *) Function ums'
+  (A : LinDec)
+  (recdepth : nat)
+  (s : Small A)
+  (sort : list A -> list A)
+  (split : Split A)
+  (l : list A)
+  {measure length l} : list A :=
+match small recdepth l with
+    | inl _ => sort l
+    | inr (h, t) =>
+        let
+          (l1, l2) := split l
+        in
+          merge A (ums' (1 + recdepth) s sort split l1,
+                   ums' (1 + recdepth) s sort split l2)
+end.
+Proof.
+  intros. apply small_inr in teq.
+Abort.
+
