Sorting/Test.v
@@ -9,13 +9,12 @@ Require Import QuickSort.
 Require Import TreeSort.
 Require Import RedblackSort.
 
-Require Import Heapsort.
 Require Import PairingSort.
 Require Import SplaySort.
 
 Require Import ListLemmas.
 
-Require Import TrichQuicksort.
+(*Require Import TrichQuicksort.*)
 
 Require Import LeftistHeap.
 
@@ -45,22 +44,19 @@ Time Compute stdSort_nat [].
 
 (* Slow sorts on small lists. *)
 
-Require Import SelectionSort2.
-
-(*Time Compute SelectionSort.ss natle (cycle 100 testl).
-Time Compute SelectionSort2.ss natle (cycle 100 testl).
-Time Compute SelectionSort2.ss' natle (cycle 100 testl).
-Time Compute SelectionSort2.ss'' natle (cycle 100 testl).
+(*Time Compute ss natle (cycle 100 testl).
+Time Compute ss' natle (cycle 100 testl).
+Time Compute ss'' natle (cycle 100 testl).
+Time Compute ss_bifilter natle (cycle 500 testl).
+Time Compute ss_mins' natlt (cycle 500 testl).
 
 Time Compute ss natle (cycle 10 testl).
 Time Compute insertionSort natle (cycle 10 testl).*)
 
 (* Fast sorts on medium lists. *)
 
-(*
-Time Eval native_compute in ms natle (cycle 100 testl).
-Time Compute ms natle (cycle 100 testl).
-Time Eval native_compute in ms2 natle (cycle 100 testl).
+(*Time Compute ms natle (cycle 100 testl).
+Time Compute ms2 natle (cycle 100 testl).
 
 Time Compute qs natle (cycle 100 testl).
 Time Compute qs2 natle (cycle 100 testl).
@@ -84,27 +80,28 @@ Time Eval lazy in pairingSort natle (cycle 100 testl).
 *)
 
 (* Fast sorts on big lists. *)
-(*Time Compute ms natle (cycle 200 testl).
+
+(*
+Time Compute ms natle (cycle 200 testl).
 Time Compute ms2 natle (cycle 200 testl).
-Time Compute ums 0 0 (treeSort natle) (MsSplit natle) (cycle 200 testl).
 
 Time Compute qs natle (cycle 200 testl).
 Time Compute qs2 natle (cycle 200 testl).
-Time Compute uqs natle (cycle 200 testl).
-
-Time Compute treeSort natle (cycle 200 testl).
-Time Compute redblackSort natle (cycle 200 testl).
+Time Compute ums 0 1 (treeSort natle) (MsSplit natle) (cycle 500 testl).
 *)
 
-(*Time Compute tqs natlt (cycle 1000 testl).
-
+(*
 Time Compute treeSort natle (cycle 1000 testl).
 Time Compute treeSort' natle (cycle 1000 testl).
+*)
 
+(*
 Time Compute redblackSort natle (cycle 1000 testl).
-Time Compute redblackSort' natle (cycle 1000 testl).
 
-Time Eval lazy in leftistHeapsort' natle (cycle 300 testl).*)
+Time Compute hqs 64 (Sort_redblackSort natle) (cycle 1000 testl).
+
+Time Eval lazy in leftistHeapsort' natle (cycle 300 testl).
+*)
 
 (* Hybrid mergesort on big lists. *)
 (*Time Compute @ghms 512 natle (insertionSort natle) (MsSplit natle)
@@ -141,26 +138,35 @@ Time Compute @htqs 1 natlt (redblackSort natle) (cycle 200 testl).*)
 (* Long lists made of one element. *)
 Definition l1 := cycle 2500 [0].
 
-(*Time Compute @ghms 64 natle (insertionSort natle) (MsSplit natle) l1.
+(*
+Time Compute @ghms 64 natle (insertionSort natle) (MsSplit natle) l1.
 
 Time Compute @ghms 64 natle (treeSort natle) (MsSplit natle) l1.
 Time Compute @ghms 64 natle (redblackSort natle) (MsSplit natle) l1.
 
-Time Compute @ghms 64 natle (leftistHeapsort' natle) (MsSplit natle) l1.
 Time Compute @ghms 64 natle (pairingSort natle) (MsSplit natle) l1.
 
-Time Compute @hqs 1024 natle (insertionSort natle) l1.
+Time Compute @hqs 1024 natle (Sort_insertionSort natle) l1.
+*)
 
-Time Compute @hqs 512 natle (treeSort natle) l1.
-Time Compute @hqs 512 natle (redblackSort natle) l1.
+(*Time Compute @hqs 512 natle (Sort_treeSort natle) l1.*)
 
-Time Compute @hqs 512 natle (pairingSort natle) l1.
+(*
+Time Compute @hqs 512 natle (Sort_redblackSort natle) l1.
 
+Time Compute @hqs 512 natle (Sort_pairingSort natle) l1.
+*)
+
+(*
 Time Compute @htqs 0 natlt (insertionSort natle) l1.
 
 Time Compute @htqs 0 natlt (treeSort natle) l1.
 
-Time Compute @htqs 0 natlt (redblackSort natle) l1.*)
+Time Compute @htqs 0 natlt (redblackSort natle) l1.
+
+Time Compute @uqs natlt (Small_head natlt) (AdHocSort_id natlt)
+                 (Pivot_head natlt) (Partition_trifilter natlt) l1.
+*)
 
 Fixpoint toN (n : nat) : list nat :=
 match n with
